\documentclass[a4paper]{article}
\usepackage{amsmath}
\usepackage{amssymb}
\usepackage{../../math_symbol}
\usepackage{../../header}

\newcommand{\thechapter}{3}
\title{Durret 5th Chapter{\thechapter} Solutions}
\author{htao}


\makeatletter
\def\thm@space@setup{\thm@preskip=0.3 \baselineskip}
\makeatother


\usepackage{physics}


\renewcommand{\theexercise}{\thechapter.\arabic{section}.\arabic{exercise}}

\renewcommand{\thetheorem}{\thechapter.\arabic{section}.\arabic{theorem}}


\begin{document}
\maketitle

\section{}

\begin{exercise}

\end{exercise}
\begin{solution}
    By the Taylor's expansion, the logritham of the sum is
    \begin{align*}
        \sum_{j=1}^{n} \ln(1+c_{j,n})& = \sum_{j=1}^{n} (c_{j,n} - \frac{1}{(1+c_{j,n})^2}c_{j,n}^2)\\
                                    &=\sum_{j=1}^{n} c_{j,n} - \sum_{j=1}^{n} \frac{1}{(1+c_{j,n})^2}c_{j,n}^2
    \end{align*}
    where $\sum_{j=1}^{n} c_{j,n} \to \lambda$.And letting $c_n := \max_{1\le j\le n} \abs{c_{j,n}}<$, for large $n$ such that $c_n<1$
    \[
        \abs{\sum_{j=1}^{n} \frac{1}{(1+c_{j,n})^2}c_{j,n}^2} \le \abs{\frac{1}{(1-c_n)^2}}\abs{c_n}\sum_{j=1}^{n}{\abs{c_{j,n}}} \to 0
    \]
    The desired result follows.
\end{solution}
\section{}
\section{}
\section{}
\section{}
\section{}
\section{}



\appendix
\section{Related Theorem Details}

\stepcounter{section}
\stepcounter{section}
\stepcounter{section}
\stepcounter{section}
\stepcounter{section}

\subsection*{2.7}

\end{document}